setup.py
@@ -1,0 +1,26 @@
+from setuptools import setup, find_packages
+
+setup(
+    name='flux-certify',
+    version='0.1.0',
+    description='Compile FLUX-C guard constraints and generate proof certificates',
+    long_description=open('README.md').read(),
+    long_description_content_type='text/markdown',
+    author='SuperInstance',
+    author_email='cocapn@example.com',
+    url='https://github.com/SuperInstance/flux-certify',
+    package_dir={'': 'src'},
+    packages=find_packages('src'),
+    python_requires='>=3.8',
+    install_requires=['click>=8.0'],
+    entry_points={
+        'console_scripts': ['flux-certify=flux_certify.cli:main'],
+    },
+    classifiers=[
+        'Development Status :: 3 - Alpha',
+        'Intended Audience :: Developers',
+        'Topic :: Software Development :: Compilers',
+        'License :: OSI Approved :: Apache Software License',
+        'Programming Language :: Python :: 3',
+    ],
+)
